Use fv to mildly restate safety

src/helpers.lean
@@ -1,6 +1,49 @@
 import statics
 import dynamics
 
+theorem subset_trans
+  {t: Type}
+  (a b c: set t)
+  (ab: a ⊆ b) (bc: b ⊆ c): a ⊆ c
+:=
+begin
+  intros _ h,
+  exact bc (ab h)
+end
+
+@[reducible]
+def fv (e: exp): set var :=
+  exp.rec_on e
+  -- int
+  (fun _, ∅)
+  -- true
+  ∅
+  -- false
+  ∅
+  -- if_
+  (fun _ _ _ s1 s2 s3, s1 ∪ s2 ∪ s3)
+
+theorem subset_if (e1 e2 e3: exp):
+  fv e1 ⊆ fv (exp.if_ e1 e2 e3) ∧
+  fv e2 ⊆ fv (exp.if_ e1 e2 e3) ∧
+  fv e3 ⊆ fv (exp.if_ e1 e2 e3) :=
+begin
+  simp [fv],
+  split,
+  intros _ a,
+  left,
+  left,
+  exact a,
+  split,
+  intros _ b,
+  left,
+  right,
+  exact b,
+  intros _ c,
+  right,
+  exact c,
+end
+
 theorem lookup_same
   (Γ: cx typ) (x: var) (τ: typ) (τ': typ)
   (l1: lookup Γ x τ)
