src/var.lean
@@ -4,6 +4,8 @@ def var: Type := string
 @[reducible]
 def cx (t: Type) := list (prod var t)
 
+def vars {t: Type} (Γ: cx t): set var := { x | x ∈ list.map prod.fst Γ }
+
 inductive lookup {t: Type}: cx t -> var -> t -> Prop
 | hd (Γ: cx t) (x: var) (out: t): lookup (list.cons (prod.mk x out) Γ) x out
 | tl (Γ: cx t) (x: var) (out: t) (y: var) (out_y: t):
