src/safety.lean
@@ -2,8 +2,9 @@ import helpers
 
 theorem progress
   (Γ: cx typ)
-  (tcx_nil: Γ = list.nil)
-  (e: exp) (τ: typ)
+  (e: exp)
+  (Γ_ok: fv e ⊆ vars Γ)
+  (τ: typ)
   (et: has_typ Γ e τ)
   : val e ∨ (∃ (e': exp), steps e e') :=
 begin
@@ -15,7 +16,14 @@ begin
   left,
   exact val.false,
   right,
-  cases et_ih_a tcx_nil,
+  let s_if := subset_if et_e1 et_e2 et_e3,
+  let hm := subset_trans
+    (fv et_e1)
+    (fv (exp.if_ et_e1 et_e2 et_e3))
+    (vars et_Γ)
+    s_if.left
+    Γ_ok,
+  cases et_ih_a hm,
   cases bool_canonical_forms et_Γ et_e1 h et_a,
   rewrite h_1,
   existsi et_e2,
@@ -30,15 +38,23 @@ end
 
 theorem preservation
   (Γ: cx typ)
-  (tcx_nil: Γ = list.nil)
-  (e: exp) (e': exp) (τ: typ)
+  (e: exp)
+  (Γ_ok: fv e ⊆ vars Γ)
+  (e': exp) (τ: typ)
   (et: has_typ Γ e τ)
   (st: steps e e')
   : has_typ Γ e' τ :=
 begin
   induction st generalizing Γ τ,
   let inv := inversion_if Γ st_e1 st_e2 st_e3 τ et,
-  let e1_typ := st_ih Γ typ.bool tcx_nil inv.left,
+  let s_if := subset_if st_e1 st_e2 st_e3,
+  let hm := subset_trans
+    (fv st_e1)
+    (fv (exp.if_ st_e1 st_e2 st_e3))
+    (vars Γ)
+    s_if.left
+    Γ_ok,
+  let e1_typ := st_ih Γ typ.bool hm inv.left,
   exact has_typ.if_ Γ st_e1' st_e2 st_e3 τ e1_typ inv.right.left inv.right.right,
   let inv := inversion_if Γ exp.true st_e2 st_e3 τ et,
   exact inv.right.left,
